update the generated files
git-svn-id: https://projects.brucker.ch/hol-testgen/svn/HOL-TestGen/trunk/hol-testgen@10367 3260e6d1-4efc-4170-b0a7-36055960796d

doc/Employee_AnalysisModel_UMLPart_generated.thy
@@ -2243,7 +2243,7 @@ lemma Planet_OclAllInstances_generic_OclIsTypeOf\<^sub>P\<^sub>l\<^sub>a\<^sub>n
 assumes [simp]: "(\<And>x. (pre_post ((x , x))) = x)"
 shows "(\<exists>\<tau>. \<tau> \<Turnstile> (not ((OclForall ((OclAllInstances_generic (pre_post) (Planet))) (OclIsTypeOf\<^sub>P\<^sub>l\<^sub>a\<^sub>n\<^sub>e\<^sub>t)))))"
   proof - fix oid a show ?thesis
-  proof - let ?t0 = "(state.make ((Map.empty (oid \<mapsto> (in\<^sub>P\<^sub>l\<^sub>a\<^sub>n\<^sub>e\<^sub>t ((mkoid\<^sub>P\<^sub>l\<^sub>a\<^sub>n\<^sub>e\<^sub>t ((mk\<^sub>P\<^sub>l\<^sub>a\<^sub>n\<^sub>e\<^sub>t_\<^sub>P\<^sub>e\<^sub>r\<^sub>s\<^sub>o\<^sub>n (a))) (None))))))) (Map.empty) (Map.empty))" show ?thesis
+  proof - let ?t0 = "(state.make ((Map.empty (oid \<mapsto> (in\<^sub>P\<^sub>l\<^sub>a\<^sub>n\<^sub>e\<^sub>t ((mkoid\<^sub>P\<^sub>l\<^sub>a\<^sub>n\<^sub>e\<^sub>t ((mk\<^sub>P\<^sub>l\<^sub>a\<^sub>n\<^sub>e\<^sub>t_\<^sub>P\<^sub>e\<^sub>r\<^sub>s\<^sub>o\<^sub>n (a))) (None))))))) (Map.empty))" show ?thesis
   apply(rule exI[where x = "(?t0 , ?t0)"], simp add: OclValid_def del: OclAllInstances_generic_def)
   apply(simp only: OclForall_def refl if_True OclAllInstances_generic_defined[simplified OclValid_def])
   apply(simp only: OclAllInstances_generic_def OclAsType\<^sub>P\<^sub>l\<^sub>a\<^sub>n\<^sub>e\<^sub>t_\<AA>_def)
@@ -2277,7 +2277,7 @@ lemma Galaxy_OclAllInstances_generic_OclIsTypeOf\<^sub>G\<^sub>a\<^sub>l\<^sub>a
 assumes [simp]: "(\<And>x. (pre_post ((x , x))) = x)"
 shows "(\<exists>\<tau>. \<tau> \<Turnstile> (not ((OclForall ((OclAllInstances_generic (pre_post) (Galaxy))) (OclIsTypeOf\<^sub>G\<^sub>a\<^sub>l\<^sub>a\<^sub>x\<^sub>y)))))"
   proof - fix oid a show ?thesis
-  proof - let ?t0 = "(state.make ((Map.empty (oid \<mapsto> (in\<^sub>G\<^sub>a\<^sub>l\<^sub>a\<^sub>x\<^sub>y ((mkoid\<^sub>G\<^sub>a\<^sub>l\<^sub>a\<^sub>x\<^sub>y ((mk\<^sub>G\<^sub>a\<^sub>l\<^sub>a\<^sub>x\<^sub>y_\<^sub>P\<^sub>l\<^sub>a\<^sub>n\<^sub>e\<^sub>t (a))) (None) (None))))))) (Map.empty) (Map.empty))" show ?thesis
+  proof - let ?t0 = "(state.make ((Map.empty (oid \<mapsto> (in\<^sub>G\<^sub>a\<^sub>l\<^sub>a\<^sub>x\<^sub>y ((mkoid\<^sub>G\<^sub>a\<^sub>l\<^sub>a\<^sub>x\<^sub>y ((mk\<^sub>G\<^sub>a\<^sub>l\<^sub>a\<^sub>x\<^sub>y_\<^sub>P\<^sub>l\<^sub>a\<^sub>n\<^sub>e\<^sub>t (a))) (None) (None))))))) (Map.empty))" show ?thesis
   apply(rule exI[where x = "(?t0 , ?t0)"], simp add: OclValid_def del: OclAllInstances_generic_def)
   apply(simp only: OclForall_def refl if_True OclAllInstances_generic_defined[simplified OclValid_def])
   apply(simp only: OclAllInstances_generic_def OclAsType\<^sub>G\<^sub>a\<^sub>l\<^sub>a\<^sub>x\<^sub>y_\<AA>_def)
@@ -2311,7 +2311,7 @@ lemma OclAny_OclAllInstances_generic_OclIsTypeOf\<^sub>O\<^sub>c\<^sub>l\<^sub>A
 assumes [simp]: "(\<And>x. (pre_post ((x , x))) = x)"
 shows "(\<exists>\<tau>. \<tau> \<Turnstile> (not ((OclForall ((OclAllInstances_generic (pre_post) (OclAny))) (OclIsTypeOf\<^sub>O\<^sub>c\<^sub>l\<^sub>A\<^sub>n\<^sub>y)))))"
   proof - fix oid a show ?thesis
-  proof - let ?t0 = "(state.make ((Map.empty (oid \<mapsto> (in\<^sub>O\<^sub>c\<^sub>l\<^sub>A\<^sub>n\<^sub>y ((mkoid\<^sub>O\<^sub>c\<^sub>l\<^sub>A\<^sub>n\<^sub>y ((mk\<^sub>O\<^sub>c\<^sub>l\<^sub>A\<^sub>n\<^sub>y_\<^sub>G\<^sub>a\<^sub>l\<^sub>a\<^sub>x\<^sub>y (a))))))))) (Map.empty) (Map.empty))" show ?thesis
+  proof - let ?t0 = "(state.make ((Map.empty (oid \<mapsto> (in\<^sub>O\<^sub>c\<^sub>l\<^sub>A\<^sub>n\<^sub>y ((mkoid\<^sub>O\<^sub>c\<^sub>l\<^sub>A\<^sub>n\<^sub>y ((mk\<^sub>O\<^sub>c\<^sub>l\<^sub>A\<^sub>n\<^sub>y_\<^sub>G\<^sub>a\<^sub>l\<^sub>a\<^sub>x\<^sub>y (a))))))))) (Map.empty))" show ?thesis
   apply(rule exI[where x = "(?t0 , ?t0)"], simp add: OclValid_def del: OclAllInstances_generic_def)
   apply(simp only: OclForall_def refl if_True OclAllInstances_generic_defined[simplified OclValid_def])
   apply(simp only: OclAllInstances_generic_def OclAsType\<^sub>O\<^sub>c\<^sub>l\<^sub>A\<^sub>n\<^sub>y_\<AA>_def)
@@ -2524,7 +2524,7 @@ pretty much similar to the \inlineisar+Employee_DesignModel_UMLPart+, where we s
 an \verb+oid+ inside the class as ``pointer.''  *}
 
 (* 101 ************************************ 630 + 1 *)
-definition "oid\<^sub>P\<^sub>e\<^sub>r\<^sub>s\<^sub>o\<^sub>n\<B>\<O>\<S>\<S> = 0"
+definition "oid\<^sub>P\<^sub>e\<^sub>r\<^sub>s\<^sub>o\<^sub>n_0_\<B>\<O>\<S>\<S> = 0"
 
 (* 102 ************************************ 631 + 1 *)
 text{* 
@@ -2545,16 +2545,19 @@ text{*
 @{text snd}, the @{text to_from}-parameter either with the identity @{term id} or
 the following combinator @{text switch}:  *}
 
-(* 105 ************************************ 637 + 6 *)
-definition "choose\<^sub>2_1 = fst"
-definition "choose\<^sub>2_2 = snd"
-definition "switch\<^sub>2_1 = id"
-definition "switch\<^sub>2_2 = (\<lambda>(x , y). (y , x))"
+(* 105 ************************************ 637 + 8 *)
+definition "choose_0 = fst"
+definition "choose_1 = snd"
+definition "switch\<^sub>2_01 = (\<lambda> [x0 , x1] \<Rightarrow> (x0 , x1))"
+definition "switch\<^sub>2_10 = (\<lambda> [x0 , x1] \<Rightarrow> (x1 , x0))"
 definition "List_flatten = (\<lambda>l. (foldl ((\<lambda>acc. (\<lambda>l. (foldl ((\<lambda>acc. (\<lambda>l. (Cons (l) (acc))))) (acc) ((rev (l))))))) (Nil) ((rev (l)))))"
-definition "deref_assocs\<^sub>2 pre_post to_from assoc_oid f oid = (\<lambda>\<tau>. (case (assocs\<^sub>2 ((pre_post (\<tau>))) (assoc_oid)) of \<lfloor>S\<rfloor> \<Rightarrow> (f ((List_flatten ((List.map (choose\<^sub>2_2 \<circ> to_from) ((filter ((\<lambda>p. (List.member (((choose\<^sub>2_1) ((to_from (p))))) (oid)))) (S))))))) (\<tau>))
+definition "map_of_list = (foldl ((\<lambda>map. (\<lambda>(x , l1). (case (map (x)) of None \<Rightarrow> (map (x \<mapsto> l1))
+    | \<lfloor>l0\<rfloor> \<Rightarrow> (map (x \<mapsto> (List_flatten ([l0 , l1])))))))) (Map.empty))"
+definition "deref_assocs_list to_from oid S = (List_flatten ((List.map (choose_1 \<circ> to_from) ((filter ((\<lambda>p. (List.member (((choose_0) ((to_from (p))))) (oid)))) (S))))))"
+definition "deref_assocs pre_post to_from assoc_oid f oid = (\<lambda>\<tau>. (case (assocs ((pre_post (\<tau>))) (assoc_oid)) of \<lfloor>S\<rfloor> \<Rightarrow> (f ((deref_assocs_list (to_from) (oid) (S))) (\<tau>))
     | _ \<Rightarrow> (invalid (\<tau>))))"
 
-(* 106 ************************************ 643 + 4 *)
+(* 106 ************************************ 645 + 4 *)
 definition "deref_oid\<^sub>P\<^sub>e\<^sub>r\<^sub>s\<^sub>o\<^sub>n fst_snd f oid = (\<lambda>\<tau>. (case (heap (fst_snd \<tau>) (oid)) of \<lfloor>in\<^sub>P\<^sub>e\<^sub>r\<^sub>s\<^sub>o\<^sub>n obj\<rfloor> \<Rightarrow> f obj \<tau>
     | _ \<Rightarrow> invalid \<tau>))"
 definition "deref_oid\<^sub>P\<^sub>l\<^sub>a\<^sub>n\<^sub>e\<^sub>t fst_snd f oid = (\<lambda>\<tau>. (case (heap (fst_snd \<tau>) (oid)) of \<lfloor>in\<^sub>P\<^sub>l\<^sub>a\<^sub>n\<^sub>e\<^sub>t obj\<rfloor> \<Rightarrow> f obj \<tau>
@@ -2564,10 +2567,10 @@ definition "deref_oid\<^sub>G\<^sub>a\<^sub>l\<^sub>a\<^sub>x\<^sub>y fst_snd f 
 definition "deref_oid\<^sub>O\<^sub>c\<^sub>l\<^sub>A\<^sub>n\<^sub>y fst_snd f oid = (\<lambda>\<tau>. (case (heap (fst_snd \<tau>) (oid)) of \<lfloor>in\<^sub>O\<^sub>c\<^sub>l\<^sub>A\<^sub>n\<^sub>y obj\<rfloor> \<Rightarrow> f obj \<tau>
     | _ \<Rightarrow> invalid \<tau>))"
 
-(* 107 ************************************ 647 + 1 *)
-definition "deref_assocs\<^sub>P\<^sub>e\<^sub>r\<^sub>s\<^sub>o\<^sub>n\<B>\<O>\<S>\<S> fst_snd f = (deref_assocs\<^sub>2 (fst_snd) (switch\<^sub>2_1) (oid\<^sub>P\<^sub>e\<^sub>r\<^sub>s\<^sub>o\<^sub>n\<B>\<O>\<S>\<S>) (f)) \<circ> oid_of"
+(* 107 ************************************ 649 + 1 *)
+definition "deref_assocs\<^sub>P\<^sub>e\<^sub>r\<^sub>s\<^sub>o\<^sub>n_0_\<B>\<O>\<S>\<S> fst_snd f = (deref_assocs (fst_snd) (switch\<^sub>2_01) (oid\<^sub>P\<^sub>e\<^sub>r\<^sub>s\<^sub>o\<^sub>n_0_\<B>\<O>\<S>\<S>) (f)) \<circ> oid_of"
 
-(* 108 ************************************ 648 + 1 *)
+(* 108 ************************************ 650 + 1 *)
 text{* 
    The continuation @{text f} is usually instantiated with a smashing
 function which is either the identity @{term id} or, for \inlineocl{0..1} cardinalities
@@ -2575,14 +2578,14 @@ of associations, the @{term OclANY}-selector which also handles the
 @{term null}-cases appropriately. A standard use-case for this combinator
 is for example:  *}
 
-(* 109 ************************************ 649 + 1 *)
+(* 109 ************************************ 651 + 1 *)
 definition "select_object mt incl smash deref l = (smash ((foldl (incl) (mt) ((List.map (deref) (l))))))"
 
-(* 110 ************************************ 650 + 1 *)
+(* 110 ************************************ 652 + 1 *)
 text{* 
    pointer undefined in state or not referencing a type conform object representation  *}
 
-(* 111 ************************************ 651 + 9 *)
+(* 111 ************************************ 653 + 9 *)
 definition "select\<^sub>P\<^sub>e\<^sub>r\<^sub>s\<^sub>o\<^sub>n\<S>\<A>\<L>\<A>\<R>\<Y> f = (\<lambda> (mkoid\<^sub>P\<^sub>e\<^sub>r\<^sub>s\<^sub>o\<^sub>n (_) (\<bottom>)) \<Rightarrow> null
     | (mkoid\<^sub>P\<^sub>e\<^sub>r\<^sub>s\<^sub>o\<^sub>n (_) (\<lfloor>salary\<rfloor>)) \<Rightarrow> (f ((\<lambda>x _. \<lfloor>\<lfloor>x\<rfloor>\<rfloor>)) (salary)))"
 definition "select\<^sub>P\<^sub>l\<^sub>a\<^sub>n\<^sub>e\<^sub>t\<W>\<E>\<I>\<G>\<H>\<T> f = (\<lambda> (mkoid\<^sub>P\<^sub>l\<^sub>a\<^sub>n\<^sub>e\<^sub>t (_) (\<bottom>)) \<Rightarrow> null
@@ -2604,12 +2607,12 @@ definition "select\<^sub>P\<^sub>l\<^sub>a\<^sub>n\<^sub>e\<^sub>t\<M>\<O>\<V>\<
     | (mkoid\<^sub>P\<^sub>l\<^sub>a\<^sub>n\<^sub>e\<^sub>t ((mk\<^sub>P\<^sub>l\<^sub>a\<^sub>n\<^sub>e\<^sub>t (_) (_) (\<lfloor>moving\<rfloor>))) (_)) \<Rightarrow> (f ((\<lambda>x _. \<lfloor>\<lfloor>x\<rfloor>\<rfloor>)) (moving))
     | (mkoid\<^sub>P\<^sub>l\<^sub>a\<^sub>n\<^sub>e\<^sub>t ((mk\<^sub>P\<^sub>l\<^sub>a\<^sub>n\<^sub>e\<^sub>t_\<^sub>P\<^sub>e\<^sub>r\<^sub>s\<^sub>o\<^sub>n (person))) (_)) \<Rightarrow> (select\<^sub>P\<^sub>e\<^sub>r\<^sub>s\<^sub>o\<^sub>n\<M>\<O>\<V>\<I>\<N>\<G> (f) (person)))"
 
-(* 112 ************************************ 660 + 1 *)
+(* 112 ************************************ 662 + 1 *)
 definition "select\<^sub>P\<^sub>e\<^sub>r\<^sub>s\<^sub>o\<^sub>n\<B>\<O>\<S>\<S> f = (select_object (mtSet) (OclIncluding) (OclANY) ((f ((\<lambda>x _. \<lfloor>\<lfloor>x\<rfloor>\<rfloor>)))))"
 
-(* 113 ************************************ 661 + 10 *)
-consts dot\<B>\<O>\<S>\<S> :: "(\<AA>, '\<alpha>) val \<Rightarrow> Person" ("(_) .boss")
-consts dot\<B>\<O>\<S>\<S>at_pre :: "(\<AA>, '\<alpha>) val \<Rightarrow> Person" ("(_) .boss@pre")
+(* 113 ************************************ 663 + 10 *)
+consts dot_0_\<B>\<O>\<S>\<S> :: "(\<AA>, '\<alpha>) val \<Rightarrow> Person" ("(_) .boss")
+consts dot_0_\<B>\<O>\<S>\<S>at_pre :: "(\<AA>, '\<alpha>) val \<Rightarrow> Person" ("(_) .boss@pre")
 consts dot\<S>\<A>\<L>\<A>\<R>\<Y> :: "(\<AA>, '\<alpha>) val \<Rightarrow> (\<AA>, int option option) val" ("(_) .salary")
 consts dot\<S>\<A>\<L>\<A>\<R>\<Y>at_pre :: "(\<AA>, '\<alpha>) val \<Rightarrow> (\<AA>, int option option) val" ("(_) .salary@pre")
 consts dot\<W>\<E>\<I>\<G>\<H>\<T> :: "(\<AA>, '\<alpha>) val \<Rightarrow> (\<AA>, nat option option) val" ("(_) .weight")
@@ -2619,10 +2622,10 @@ consts dot\<S>\<O>\<U>\<N>\<D>at_pre :: "(\<AA>, '\<alpha>) val \<Rightarrow> (\
 consts dot\<M>\<O>\<V>\<I>\<N>\<G> :: "(\<AA>, '\<alpha>) val \<Rightarrow> (\<AA>, bool option option) val" ("(_) .moving")
 consts dot\<M>\<O>\<V>\<I>\<N>\<G>at_pre :: "(\<AA>, '\<alpha>) val \<Rightarrow> (\<AA>, bool option option) val" ("(_) .moving@pre")
 
-(* 114 ************************************ 671 + 20 *)
-defs(overloaded) dot\<^sub>P\<^sub>e\<^sub>r\<^sub>s\<^sub>o\<^sub>n\<B>\<O>\<S>\<S> : "(x::Person) .boss \<equiv> (eval_extract (x) ((deref_oid\<^sub>P\<^sub>e\<^sub>r\<^sub>s\<^sub>o\<^sub>n (in_post_state) ((deref_assocs\<^sub>P\<^sub>e\<^sub>r\<^sub>s\<^sub>o\<^sub>n\<B>\<O>\<S>\<S> (in_post_state) ((select\<^sub>P\<^sub>e\<^sub>r\<^sub>s\<^sub>o\<^sub>n\<B>\<O>\<S>\<S> ((deref_oid\<^sub>P\<^sub>e\<^sub>r\<^sub>s\<^sub>o\<^sub>n (in_post_state))))))))))"
+(* 114 ************************************ 673 + 20 *)
+defs(overloaded) dot\<^sub>P\<^sub>e\<^sub>r\<^sub>s\<^sub>o\<^sub>n_0_\<B>\<O>\<S>\<S> : "(x::Person) .boss \<equiv> (eval_extract (x) ((deref_oid\<^sub>P\<^sub>e\<^sub>r\<^sub>s\<^sub>o\<^sub>n (in_post_state) ((deref_assocs\<^sub>P\<^sub>e\<^sub>r\<^sub>s\<^sub>o\<^sub>n_0_\<B>\<O>\<S>\<S> (in_post_state) ((select\<^sub>P\<^sub>e\<^sub>r\<^sub>s\<^sub>o\<^sub>n\<B>\<O>\<S>\<S> ((deref_oid\<^sub>P\<^sub>e\<^sub>r\<^sub>s\<^sub>o\<^sub>n (in_post_state))))))))))"
 defs(overloaded) dot\<^sub>P\<^sub>e\<^sub>r\<^sub>s\<^sub>o\<^sub>n\<S>\<A>\<L>\<A>\<R>\<Y> : "(x::Person) .salary \<equiv> (eval_extract (x) ((deref_oid\<^sub>P\<^sub>e\<^sub>r\<^sub>s\<^sub>o\<^sub>n (in_post_state) ((select\<^sub>P\<^sub>e\<^sub>r\<^sub>s\<^sub>o\<^sub>n\<S>\<A>\<L>\<A>\<R>\<Y> (reconst_basetype))))))"
-defs(overloaded) dot\<^sub>P\<^sub>e\<^sub>r\<^sub>s\<^sub>o\<^sub>n\<B>\<O>\<S>\<S>at_pre : "(x::Person) .boss@pre \<equiv> (eval_extract (x) ((deref_oid\<^sub>P\<^sub>e\<^sub>r\<^sub>s\<^sub>o\<^sub>n (in_pre_state) ((deref_assocs\<^sub>P\<^sub>e\<^sub>r\<^sub>s\<^sub>o\<^sub>n\<B>\<O>\<S>\<S> (in_pre_state) ((select\<^sub>P\<^sub>e\<^sub>r\<^sub>s\<^sub>o\<^sub>n\<B>\<O>\<S>\<S> ((deref_oid\<^sub>P\<^sub>e\<^sub>r\<^sub>s\<^sub>o\<^sub>n (in_pre_state))))))))))"
+defs(overloaded) dot\<^sub>P\<^sub>e\<^sub>r\<^sub>s\<^sub>o\<^sub>n_0_\<B>\<O>\<S>\<S>at_pre : "(x::Person) .boss@pre \<equiv> (eval_extract (x) ((deref_oid\<^sub>P\<^sub>e\<^sub>r\<^sub>s\<^sub>o\<^sub>n (in_pre_state) ((deref_assocs\<^sub>P\<^sub>e\<^sub>r\<^sub>s\<^sub>o\<^sub>n_0_\<B>\<O>\<S>\<S> (in_pre_state) ((select\<^sub>P\<^sub>e\<^sub>r\<^sub>s\<^sub>o\<^sub>n\<B>\<O>\<S>\<S> ((deref_oid\<^sub>P\<^sub>e\<^sub>r\<^sub>s\<^sub>o\<^sub>n (in_pre_state))))))))))"
 defs(overloaded) dot\<^sub>P\<^sub>e\<^sub>r\<^sub>s\<^sub>o\<^sub>n\<S>\<A>\<L>\<A>\<R>\<Y>at_pre : "(x::Person) .salary@pre \<equiv> (eval_extract (x) ((deref_oid\<^sub>P\<^sub>e\<^sub>r\<^sub>s\<^sub>o\<^sub>n (in_pre_state) ((select\<^sub>P\<^sub>e\<^sub>r\<^sub>s\<^sub>o\<^sub>n\<S>\<A>\<L>\<A>\<R>\<Y> (reconst_basetype))))))"
 defs(overloaded) dot\<^sub>P\<^sub>l\<^sub>a\<^sub>n\<^sub>e\<^sub>t\<W>\<E>\<I>\<G>\<H>\<T> : "(x::Planet) .weight \<equiv> (eval_extract (x) ((deref_oid\<^sub>P\<^sub>l\<^sub>a\<^sub>n\<^sub>e\<^sub>t (in_post_state) ((select\<^sub>P\<^sub>l\<^sub>a\<^sub>n\<^sub>e\<^sub>t\<W>\<E>\<I>\<G>\<H>\<T> (reconst_basetype))))))"
 defs(overloaded) dot\<^sub>P\<^sub>l\<^sub>a\<^sub>n\<^sub>e\<^sub>t\<W>\<E>\<I>\<G>\<H>\<T>at_pre : "(x::Planet) .weight@pre \<equiv> (eval_extract (x) ((deref_oid\<^sub>P\<^sub>l\<^sub>a\<^sub>n\<^sub>e\<^sub>t (in_pre_state) ((select\<^sub>P\<^sub>l\<^sub>a\<^sub>n\<^sub>e\<^sub>t\<W>\<E>\<I>\<G>\<H>\<T> (reconst_basetype))))))"
@@ -2641,10 +2644,10 @@ defs(overloaded) dot\<^sub>P\<^sub>l\<^sub>a\<^sub>n\<^sub>e\<^sub>t\<M>\<O>\<V>
 defs(overloaded) dot\<^sub>P\<^sub>l\<^sub>a\<^sub>n\<^sub>e\<^sub>t\<S>\<O>\<U>\<N>\<D>at_pre : "(x::Planet) .sound@pre \<equiv> (eval_extract (x) ((deref_oid\<^sub>P\<^sub>l\<^sub>a\<^sub>n\<^sub>e\<^sub>t (in_pre_state) ((select\<^sub>P\<^sub>l\<^sub>a\<^sub>n\<^sub>e\<^sub>t\<S>\<O>\<U>\<N>\<D> (reconst_basetype))))))"
 defs(overloaded) dot\<^sub>P\<^sub>l\<^sub>a\<^sub>n\<^sub>e\<^sub>t\<M>\<O>\<V>\<I>\<N>\<G>at_pre : "(x::Planet) .moving@pre \<equiv> (eval_extract (x) ((deref_oid\<^sub>P\<^sub>l\<^sub>a\<^sub>n\<^sub>e\<^sub>t (in_pre_state) ((select\<^sub>P\<^sub>l\<^sub>a\<^sub>n\<^sub>e\<^sub>t\<M>\<O>\<V>\<I>\<N>\<G> (reconst_basetype))))))"
 
-(* 115 ************************************ 691 + 1 *)
-lemmas [simp,code_unfold] = dot\<^sub>P\<^sub>e\<^sub>r\<^sub>s\<^sub>o\<^sub>n\<B>\<O>\<S>\<S>
+(* 115 ************************************ 693 + 1 *)
+lemmas [simp,code_unfold] = dot\<^sub>P\<^sub>e\<^sub>r\<^sub>s\<^sub>o\<^sub>n_0_\<B>\<O>\<S>\<S>
                             dot\<^sub>P\<^sub>e\<^sub>r\<^sub>s\<^sub>o\<^sub>n\<S>\<A>\<L>\<A>\<R>\<Y>
-                            dot\<^sub>P\<^sub>e\<^sub>r\<^sub>s\<^sub>o\<^sub>n\<B>\<O>\<S>\<S>at_pre
+                            dot\<^sub>P\<^sub>e\<^sub>r\<^sub>s\<^sub>o\<^sub>n_0_\<B>\<O>\<S>\<S>at_pre
                             dot\<^sub>P\<^sub>e\<^sub>r\<^sub>s\<^sub>o\<^sub>n\<S>\<A>\<L>\<A>\<R>\<Y>at_pre
                             dot\<^sub>P\<^sub>l\<^sub>a\<^sub>n\<^sub>e\<^sub>t\<W>\<E>\<I>\<G>\<H>\<T>
                             dot\<^sub>P\<^sub>l\<^sub>a\<^sub>n\<^sub>e\<^sub>t\<W>\<E>\<I>\<G>\<H>\<T>at_pre
@@ -2663,18 +2666,18 @@ lemmas [simp,code_unfold] = dot\<^sub>P\<^sub>e\<^sub>r\<^sub>s\<^sub>o\<^sub>n\
                             dot\<^sub>P\<^sub>l\<^sub>a\<^sub>n\<^sub>e\<^sub>t\<S>\<O>\<U>\<N>\<D>at_pre
                             dot\<^sub>P\<^sub>l\<^sub>a\<^sub>n\<^sub>e\<^sub>t\<M>\<O>\<V>\<I>\<N>\<G>at_pre
 
-(* 116 ************************************ 692 + 1 *)
+(* 116 ************************************ 694 + 1 *)
 subsection{* Context Passing *}
 
-(* 117 ************************************ 693 + 1 *)
+(* 117 ************************************ 695 + 1 *)
 lemmas [simp,code_unfold] = eval_extract_def
 
-(* 118 ************************************ 694 + 20 *)
-lemma cp_dot\<^sub>P\<^sub>e\<^sub>r\<^sub>s\<^sub>o\<^sub>n\<B>\<O>\<S>\<S> : "(cp ((\<lambda>X. (X::Person) .boss)))"
+(* 118 ************************************ 696 + 20 *)
+lemma cp_dot\<^sub>P\<^sub>e\<^sub>r\<^sub>s\<^sub>o\<^sub>n_0_\<B>\<O>\<S>\<S> : "(cp ((\<lambda>X. (X::Person) .boss)))"
 by(auto simp: cp_def)
 lemma cp_dot\<^sub>P\<^sub>e\<^sub>r\<^sub>s\<^sub>o\<^sub>n\<S>\<A>\<L>\<A>\<R>\<Y> : "(cp ((\<lambda>X. (X::Person) .salary)))"
 by(auto simp: cp_def)
-lemma cp_dot\<^sub>P\<^sub>e\<^sub>r\<^sub>s\<^sub>o\<^sub>n\<B>\<O>\<S>\<S>at_pre : "(cp ((\<lambda>X. (X::Person) .boss@pre)))"
+lemma cp_dot\<^sub>P\<^sub>e\<^sub>r\<^sub>s\<^sub>o\<^sub>n_0_\<B>\<O>\<S>\<S>at_pre : "(cp ((\<lambda>X. (X::Person) .boss@pre)))"
 by(auto simp: cp_def)
 lemma cp_dot\<^sub>P\<^sub>e\<^sub>r\<^sub>s\<^sub>o\<^sub>n\<S>\<A>\<L>\<A>\<R>\<Y>at_pre : "(cp ((\<lambda>X. (X::Person) .salary@pre)))"
 by(auto simp: cp_def)
@@ -2711,10 +2714,10 @@ by(auto simp: cp_def)
 lemma cp_dot\<^sub>P\<^sub>l\<^sub>a\<^sub>n\<^sub>e\<^sub>t\<M>\<O>\<V>\<I>\<N>\<G>at_pre : "(cp ((\<lambda>X. (X::Planet) .moving@pre)))"
 by(auto simp: cp_def)
 
-(* 119 ************************************ 714 + 1 *)
-lemmas [simp,code_unfold] = cp_dot\<^sub>P\<^sub>e\<^sub>r\<^sub>s\<^sub>o\<^sub>n\<B>\<O>\<S>\<S>
+(* 119 ************************************ 716 + 1 *)
+lemmas [simp,code_unfold] = cp_dot\<^sub>P\<^sub>e\<^sub>r\<^sub>s\<^sub>o\<^sub>n_0_\<B>\<O>\<S>\<S>
                             cp_dot\<^sub>P\<^sub>e\<^sub>r\<^sub>s\<^sub>o\<^sub>n\<S>\<A>\<L>\<A>\<R>\<Y>
-                            cp_dot\<^sub>P\<^sub>e\<^sub>r\<^sub>s\<^sub>o\<^sub>n\<B>\<O>\<S>\<S>at_pre
+                            cp_dot\<^sub>P\<^sub>e\<^sub>r\<^sub>s\<^sub>o\<^sub>n_0_\<B>\<O>\<S>\<S>at_pre
                             cp_dot\<^sub>P\<^sub>e\<^sub>r\<^sub>s\<^sub>o\<^sub>n\<S>\<A>\<L>\<A>\<R>\<Y>at_pre
                             cp_dot\<^sub>P\<^sub>l\<^sub>a\<^sub>n\<^sub>e\<^sub>t\<W>\<E>\<I>\<G>\<H>\<T>
                             cp_dot\<^sub>P\<^sub>l\<^sub>a\<^sub>n\<^sub>e\<^sub>t\<W>\<E>\<I>\<G>\<H>\<T>at_pre
@@ -2733,21 +2736,21 @@ lemmas [simp,code_unfold] = cp_dot\<^sub>P\<^sub>e\<^sub>r\<^sub>s\<^sub>o\<^sub
                             cp_dot\<^sub>P\<^sub>l\<^sub>a\<^sub>n\<^sub>e\<^sub>t\<S>\<O>\<U>\<N>\<D>at_pre
                             cp_dot\<^sub>P\<^sub>l\<^sub>a\<^sub>n\<^sub>e\<^sub>t\<M>\<O>\<V>\<I>\<N>\<G>at_pre
 
-(* 120 ************************************ 715 + 1 *)
+(* 120 ************************************ 717 + 1 *)
 subsection{* Execution with Invalid or Null as Argument *}
 
-(* 121 ************************************ 716 + 40 *)
-lemma dot\<^sub>P\<^sub>e\<^sub>r\<^sub>s\<^sub>o\<^sub>n\<B>\<O>\<S>\<S>_invalid : "(invalid::Person) .boss = invalid"
+(* 121 ************************************ 718 + 40 *)
+lemma dot\<^sub>P\<^sub>e\<^sub>r\<^sub>s\<^sub>o\<^sub>n_0_\<B>\<O>\<S>\<S>_invalid : "(invalid::Person) .boss = invalid"
 by(rule ext, simp add: bot_option_def invalid_def)
-lemma dot\<^sub>P\<^sub>e\<^sub>r\<^sub>s\<^sub>o\<^sub>n\<B>\<O>\<S>\<S>_null : "(null::Person) .boss = invalid"
+lemma dot\<^sub>P\<^sub>e\<^sub>r\<^sub>s\<^sub>o\<^sub>n_0_\<B>\<O>\<S>\<S>_null : "(null::Person) .boss = invalid"
 by(rule ext, simp add: bot_option_def null_fun_def null_option_def)
 lemma dot\<^sub>P\<^sub>e\<^sub>r\<^sub>s\<^sub>o\<^sub>n\<S>\<A>\<L>\<A>\<R>\<Y>_invalid : "(invalid::Person) .salary = invalid"
 by(rule ext, simp add: bot_option_def invalid_def)
 lemma dot\<^sub>P\<^sub>e\<^sub>r\<^sub>s\<^sub>o\<^sub>n\<S>\<A>\<L>\<A>\<R>\<Y>_null : "(null::Person) .salary = invalid"
 by(rule ext, simp add: bot_option_def null_fun_def null_option_def)
-lemma dot\<^sub>P\<^sub>e\<^sub>r\<^sub>s\<^sub>o\<^sub>n\<B>\<O>\<S>\<S>at_pre_invalid : "(invalid::Person) .boss@pre = invalid"
+lemma dot\<^sub>P\<^sub>e\<^sub>r\<^sub>s\<^sub>o\<^sub>n_0_\<B>\<O>\<S>\<S>at_pre_invalid : "(invalid::Person) .boss@pre = invalid"
 by(rule ext, simp add: bot_option_def invalid_def)
-lemma dot\<^sub>P\<^sub>e\<^sub>r\<^sub>s\<^sub>o\<^sub>n\<B>\<O>\<S>\<S>at_pre_null : "(null::Person) .boss@pre = invalid"
+lemma dot\<^sub>P\<^sub>e\<^sub>r\<^sub>s\<^sub>o\<^sub>n_0_\<B>\<O>\<S>\<S>at_pre_null : "(null::Person) .boss@pre = invalid"
 by(rule ext, simp add: bot_option_def null_fun_def null_option_def)
 lemma dot\<^sub>P\<^sub>e\<^sub>r\<^sub>s\<^sub>o\<^sub>n\<S>\<A>\<L>\<A>\<R>\<Y>at_pre_invalid : "(invalid::Person) .salary@pre = invalid"
 by(rule ext, simp add: bot_option_def invalid_def)
@@ -2818,13 +2821,13 @@ by(rule ext, simp add: bot_option_def invalid_def)
 lemma dot\<^sub>P\<^sub>l\<^sub>a\<^sub>n\<^sub>e\<^sub>t\<M>\<O>\<V>\<I>\<N>\<G>at_pre_null : "(null::Planet) .moving@pre = invalid"
 by(rule ext, simp add: bot_option_def null_fun_def null_option_def)
 
-(* 122 ************************************ 756 + 1 *)
+(* 122 ************************************ 758 + 1 *)
 section{* A Little Infra-structure on Example States *}
 
-(* 123 ************************************ 757 + 1 *)
+(* 123 ************************************ 759 + 1 *)
 text{*  *}
 
-(* 124 ************************************ 758 + 1 *)
+(* 124 ************************************ 760 + 1 *)
 text{* 
 
 The example we are defining in this section comes from the figure~\ref{fig:eam1_system-states}.
@@ -2836,11 +2839,11 @@ The example we are defining in this section comes from the figure~\ref{fig:eam1_
 \end{figure}
  *}
 
-(* 125 ************************************ 759 + 1 *)
+(* 125 ************************************ 761 + 1 *)
 lemmas [simp,code_unfold] = state.defs
                             const_ss
 
-(* 126 ************************************ 760 + 1 *)
+(* 126 ************************************ 762 + 1 *)
 lemmas [simp,code_unfold] = OclAsType\<^sub>P\<^sub>e\<^sub>r\<^sub>s\<^sub>o\<^sub>n_Planet
                             OclAsType\<^sub>P\<^sub>e\<^sub>r\<^sub>s\<^sub>o\<^sub>n_Galaxy
                             OclAsType\<^sub>P\<^sub>e\<^sub>r\<^sub>s\<^sub>o\<^sub>n_OclAny
@@ -2854,7 +2857,7 @@ lemmas [simp,code_unfold] = OclAsType\<^sub>P\<^sub>e\<^sub>r\<^sub>s\<^sub>o\<^
                             OclAsType\<^sub>O\<^sub>c\<^sub>l\<^sub>A\<^sub>n\<^sub>y_Planet
                             OclAsType\<^sub>O\<^sub>c\<^sub>l\<^sub>A\<^sub>n\<^sub>y_Galaxy
 
-(* 127 ************************************ 761 + 8 *)
+(* 127 ************************************ 763 + 8 *)
 definition OclInt1000 ("\<one>\<zero>\<zero>\<zero>")
   where "OclInt1000 = (\<lambda>_. \<lfloor>\<lfloor>1000\<rfloor>\<rfloor>)"
 definition OclInt1200 ("\<one>\<two>\<zero>\<zero>")
@@ -2872,7 +2875,7 @@ definition OclInt3200 ("\<three>\<two>\<zero>\<zero>")
 definition OclInt3500 ("\<three>\<five>\<zero>\<zero>")
   where "OclInt3500 = (\<lambda>_. \<lfloor>\<lfloor>3500\<rfloor>\<rfloor>)"
 
-(* 128 ************************************ 769 + 27 *)
+(* 128 ************************************ 771 + 9 *)
 definition "oid1 = 1"
 definition "oid2 = 2"
 definition "oid3 = 3"
@@ -2882,6 +2885,8 @@ definition "oid6 = 6"
 definition "oid7 = 7"
 definition "oid8 = 8"
 definition "oid9 = 9"
+
+(* 129 ************************************ 780 + 18 *)
 definition "X\<^sub>P\<^sub>e\<^sub>r\<^sub>s\<^sub>o\<^sub>n1\<^sub>P\<^sub>e\<^sub>r\<^sub>s\<^sub>o\<^sub>n = (mkoid\<^sub>P\<^sub>e\<^sub>r\<^sub>s\<^sub>o\<^sub>n ((mk\<^sub>P\<^sub>e\<^sub>r\<^sub>s\<^sub>o\<^sub>n (oid1) (None) (None) (None))) (\<lfloor>1300\<rfloor>))"
 definition "X\<^sub>P\<^sub>e\<^sub>r\<^sub>s\<^sub>o\<^sub>n2\<^sub>P\<^sub>e\<^sub>r\<^sub>s\<^sub>o\<^sub>n = (mkoid\<^sub>P\<^sub>e\<^sub>r\<^sub>s\<^sub>o\<^sub>n ((mk\<^sub>P\<^sub>e\<^sub>r\<^sub>s\<^sub>o\<^sub>n (oid2) (None) (None) (None))) (\<lfloor>1800\<rfloor>))"
 definition "X\<^sub>P\<^sub>e\<^sub>r\<^sub>s\<^sub>o\<^sub>n3\<^sub>P\<^sub>e\<^sub>r\<^sub>s\<^sub>o\<^sub>n = (mkoid\<^sub>P\<^sub>e\<^sub>r\<^sub>s\<^sub>o\<^sub>n ((mk\<^sub>P\<^sub>e\<^sub>r\<^sub>s\<^sub>o\<^sub>n (oid3) (None) (None) (None))) (None))"
@@ -2901,18 +2906,22 @@ definition "(X\<^sub>P\<^sub>e\<^sub>r\<^sub>s\<^sub>o\<^sub>n7::OclAny) = (\<la
 definition "(X\<^sub>P\<^sub>e\<^sub>r\<^sub>s\<^sub>o\<^sub>n8::OclAny) = (\<lambda>_. \<lfloor>\<lfloor>X\<^sub>P\<^sub>e\<^sub>r\<^sub>s\<^sub>o\<^sub>n8\<^sub>O\<^sub>c\<^sub>l\<^sub>A\<^sub>n\<^sub>y\<rfloor>\<rfloor>)"
 definition "(X\<^sub>P\<^sub>e\<^sub>r\<^sub>s\<^sub>o\<^sub>n9::Person) = (\<lambda>_. \<lfloor>\<lfloor>X\<^sub>P\<^sub>e\<^sub>r\<^sub>s\<^sub>o\<^sub>n9\<^sub>P\<^sub>e\<^sub>r\<^sub>s\<^sub>o\<^sub>n\<rfloor>\<rfloor>)"
 
-(* 129 ************************************ 796 + 1 *)
-definition "\<sigma>\<^sub>1 = (state.make ((Map.empty (oid1 \<mapsto> (in\<^sub>P\<^sub>e\<^sub>r\<^sub>s\<^sub>o\<^sub>n ((mkoid\<^sub>P\<^sub>e\<^sub>r\<^sub>s\<^sub>o\<^sub>n ((mk\<^sub>P\<^sub>e\<^sub>r\<^sub>s\<^sub>o\<^sub>n (oid1) (None) (None) (None))) (\<lfloor>1000\<rfloor>))))) (oid2 \<mapsto> (in\<^sub>P\<^sub>e\<^sub>r\<^sub>s\<^sub>o\<^sub>n ((mkoid\<^sub>P\<^sub>e\<^sub>r\<^sub>s\<^sub>o\<^sub>n ((mk\<^sub>P\<^sub>e\<^sub>r\<^sub>s\<^sub>o\<^sub>n (oid2) (None) (None) (None))) (\<lfloor>1200\<rfloor>))))) (oid4 \<mapsto> (in\<^sub>P\<^sub>e\<^sub>r\<^sub>s\<^sub>o\<^sub>n ((mkoid\<^sub>P\<^sub>e\<^sub>r\<^sub>s\<^sub>o\<^sub>n ((mk\<^sub>P\<^sub>e\<^sub>r\<^sub>s\<^sub>o\<^sub>n (oid4) (None) (None) (None))) (\<lfloor>2600\<rfloor>))))) (oid5 \<mapsto> (in\<^sub>P\<^sub>e\<^sub>r\<^sub>s\<^sub>o\<^sub>n (X\<^sub>P\<^sub>e\<^sub>r\<^sub>s\<^sub>o\<^sub>n5\<^sub>P\<^sub>e\<^sub>r\<^sub>s\<^sub>o\<^sub>n))) (oid6 \<mapsto> (in\<^sub>P\<^sub>e\<^sub>r\<^sub>s\<^sub>o\<^sub>n ((mkoid\<^sub>P\<^sub>e\<^sub>r\<^sub>s\<^sub>o\<^sub>n ((mk\<^sub>P\<^sub>e\<^sub>r\<^sub>s\<^sub>o\<^sub>n (oid6) (None) (None) (None))) (\<lfloor>2300\<rfloor>))))) (oid9 \<mapsto> (in\<^sub>P\<^sub>e\<^sub>r\<^sub>s\<^sub>o\<^sub>n (X\<^sub>P\<^sub>e\<^sub>r\<^sub>s\<^sub>o\<^sub>n9\<^sub>P\<^sub>e\<^sub>r\<^sub>s\<^sub>o\<^sub>n))))) ((Map.empty (oid\<^sub>P\<^sub>e\<^sub>r\<^sub>s\<^sub>o\<^sub>n\<B>\<O>\<S>\<S> \<mapsto> (Cons ((Pair ((Cons (oid1) (Nil))) ((Cons (oid2) (Nil))))) ((Cons ((Pair ((Cons (oid4) (Nil))) ((Cons (oid5) (Nil))))) ((Cons ((Pair ((Cons (oid6) (Nil))) ((Cons (oid4) (Nil))))) (Nil))))))))) ((Map.empty )))"
+(* 130 ************************************ 798 + 0 *)
 
-(* 130 ************************************ 797 + 1 *)
+(* 131 ************************************ 798 + 1 *)
+definition "\<sigma>\<^sub>1 = (state.make ((Map.empty (oid1 \<mapsto> (in\<^sub>P\<^sub>e\<^sub>r\<^sub>s\<^sub>o\<^sub>n ((mkoid\<^sub>P\<^sub>e\<^sub>r\<^sub>s\<^sub>o\<^sub>n ((mk\<^sub>P\<^sub>e\<^sub>r\<^sub>s\<^sub>o\<^sub>n (oid1) (None) (None) (None))) (\<lfloor>1000\<rfloor>))))) (oid2 \<mapsto> (in\<^sub>P\<^sub>e\<^sub>r\<^sub>s\<^sub>o\<^sub>n ((mkoid\<^sub>P\<^sub>e\<^sub>r\<^sub>s\<^sub>o\<^sub>n ((mk\<^sub>P\<^sub>e\<^sub>r\<^sub>s\<^sub>o\<^sub>n (oid2) (None) (None) (None))) (\<lfloor>1200\<rfloor>))))) (oid4 \<mapsto> (in\<^sub>P\<^sub>e\<^sub>r\<^sub>s\<^sub>o\<^sub>n ((mkoid\<^sub>P\<^sub>e\<^sub>r\<^sub>s\<^sub>o\<^sub>n ((mk\<^sub>P\<^sub>e\<^sub>r\<^sub>s\<^sub>o\<^sub>n (oid4) (None) (None) (None))) (\<lfloor>2600\<rfloor>))))) (oid5 \<mapsto> (in\<^sub>P\<^sub>e\<^sub>r\<^sub>s\<^sub>o\<^sub>n (X\<^sub>P\<^sub>e\<^sub>r\<^sub>s\<^sub>o\<^sub>n5\<^sub>P\<^sub>e\<^sub>r\<^sub>s\<^sub>o\<^sub>n))) (oid6 \<mapsto> (in\<^sub>P\<^sub>e\<^sub>r\<^sub>s\<^sub>o\<^sub>n ((mkoid\<^sub>P\<^sub>e\<^sub>r\<^sub>s\<^sub>o\<^sub>n ((mk\<^sub>P\<^sub>e\<^sub>r\<^sub>s\<^sub>o\<^sub>n (oid6) (None) (None) (None))) (\<lfloor>2300\<rfloor>))))) (oid9 \<mapsto> (in\<^sub>P\<^sub>e\<^sub>r\<^sub>s\<^sub>o\<^sub>n (X\<^sub>P\<^sub>e\<^sub>r\<^sub>s\<^sub>o\<^sub>n9\<^sub>P\<^sub>e\<^sub>r\<^sub>s\<^sub>o\<^sub>n))))) ((map_of_list ([(oid\<^sub>P\<^sub>e\<^sub>r\<^sub>s\<^sub>o\<^sub>n_0_\<B>\<O>\<S>\<S> , (List.map ((\<lambda>(x , y). [x , y]) o switch\<^sub>2_01) ([[[oid1] , [oid2]] , [[oid4] , [oid5]] , [[oid6] , [oid4]]])))]))))"
+
+(* 132 ************************************ 799 + 0 *)
+
+(* 133 ************************************ 799 + 1 *)
 lemma dom_\<sigma>\<^sub>1 : "(dom ((heap (\<sigma>\<^sub>1)))) = {oid1 , oid2 , oid4 , oid5 , oid6 , oid9}"
 by(auto simp: \<sigma>\<^sub>1_def)
 
-(* 131 ************************************ 798 + 1 *)
+(* 134 ************************************ 800 + 1 *)
 lemmas [simp,code_unfold] = dom_\<sigma>\<^sub>1
 
-(* 132 ************************************ 799 + 1 *)
-lemma perm_\<sigma>\<^sub>1 : "\<sigma>\<^sub>1 = (state.make ((Map.empty (oid9 \<mapsto> (in\<^sub>P\<^sub>e\<^sub>r\<^sub>s\<^sub>o\<^sub>n (X\<^sub>P\<^sub>e\<^sub>r\<^sub>s\<^sub>o\<^sub>n9\<^sub>P\<^sub>e\<^sub>r\<^sub>s\<^sub>o\<^sub>n))) (oid6 \<mapsto> (in\<^sub>P\<^sub>e\<^sub>r\<^sub>s\<^sub>o\<^sub>n ((mkoid\<^sub>P\<^sub>e\<^sub>r\<^sub>s\<^sub>o\<^sub>n ((mk\<^sub>P\<^sub>e\<^sub>r\<^sub>s\<^sub>o\<^sub>n (oid6) (None) (None) (None))) (\<lfloor>2300\<rfloor>))))) (oid5 \<mapsto> (in\<^sub>P\<^sub>e\<^sub>r\<^sub>s\<^sub>o\<^sub>n (X\<^sub>P\<^sub>e\<^sub>r\<^sub>s\<^sub>o\<^sub>n5\<^sub>P\<^sub>e\<^sub>r\<^sub>s\<^sub>o\<^sub>n))) (oid4 \<mapsto> (in\<^sub>P\<^sub>e\<^sub>r\<^sub>s\<^sub>o\<^sub>n ((mkoid\<^sub>P\<^sub>e\<^sub>r\<^sub>s\<^sub>o\<^sub>n ((mk\<^sub>P\<^sub>e\<^sub>r\<^sub>s\<^sub>o\<^sub>n (oid4) (None) (None) (None))) (\<lfloor>2600\<rfloor>))))) (oid2 \<mapsto> (in\<^sub>P\<^sub>e\<^sub>r\<^sub>s\<^sub>o\<^sub>n ((mkoid\<^sub>P\<^sub>e\<^sub>r\<^sub>s\<^sub>o\<^sub>n ((mk\<^sub>P\<^sub>e\<^sub>r\<^sub>s\<^sub>o\<^sub>n (oid2) (None) (None) (None))) (\<lfloor>1200\<rfloor>))))) (oid1 \<mapsto> (in\<^sub>P\<^sub>e\<^sub>r\<^sub>s\<^sub>o\<^sub>n ((mkoid\<^sub>P\<^sub>e\<^sub>r\<^sub>s\<^sub>o\<^sub>n ((mk\<^sub>P\<^sub>e\<^sub>r\<^sub>s\<^sub>o\<^sub>n (oid1) (None) (None) (None))) (\<lfloor>1000\<rfloor>))))))) ((assocs\<^sub>2 (\<sigma>\<^sub>1))) ((assocs\<^sub>3 (\<sigma>\<^sub>1))))"
+(* 135 ************************************ 801 + 1 *)
+lemma perm_\<sigma>\<^sub>1 : "\<sigma>\<^sub>1 = (state.make ((Map.empty (oid9 \<mapsto> (in\<^sub>P\<^sub>e\<^sub>r\<^sub>s\<^sub>o\<^sub>n (X\<^sub>P\<^sub>e\<^sub>r\<^sub>s\<^sub>o\<^sub>n9\<^sub>P\<^sub>e\<^sub>r\<^sub>s\<^sub>o\<^sub>n))) (oid6 \<mapsto> (in\<^sub>P\<^sub>e\<^sub>r\<^sub>s\<^sub>o\<^sub>n ((mkoid\<^sub>P\<^sub>e\<^sub>r\<^sub>s\<^sub>o\<^sub>n ((mk\<^sub>P\<^sub>e\<^sub>r\<^sub>s\<^sub>o\<^sub>n (oid6) (None) (None) (None))) (\<lfloor>2300\<rfloor>))))) (oid5 \<mapsto> (in\<^sub>P\<^sub>e\<^sub>r\<^sub>s\<^sub>o\<^sub>n (X\<^sub>P\<^sub>e\<^sub>r\<^sub>s\<^sub>o\<^sub>n5\<^sub>P\<^sub>e\<^sub>r\<^sub>s\<^sub>o\<^sub>n))) (oid4 \<mapsto> (in\<^sub>P\<^sub>e\<^sub>r\<^sub>s\<^sub>o\<^sub>n ((mkoid\<^sub>P\<^sub>e\<^sub>r\<^sub>s\<^sub>o\<^sub>n ((mk\<^sub>P\<^sub>e\<^sub>r\<^sub>s\<^sub>o\<^sub>n (oid4) (None) (None) (None))) (\<lfloor>2600\<rfloor>))))) (oid2 \<mapsto> (in\<^sub>P\<^sub>e\<^sub>r\<^sub>s\<^sub>o\<^sub>n ((mkoid\<^sub>P\<^sub>e\<^sub>r\<^sub>s\<^sub>o\<^sub>n ((mk\<^sub>P\<^sub>e\<^sub>r\<^sub>s\<^sub>o\<^sub>n (oid2) (None) (None) (None))) (\<lfloor>1200\<rfloor>))))) (oid1 \<mapsto> (in\<^sub>P\<^sub>e\<^sub>r\<^sub>s\<^sub>o\<^sub>n ((mkoid\<^sub>P\<^sub>e\<^sub>r\<^sub>s\<^sub>o\<^sub>n ((mk\<^sub>P\<^sub>e\<^sub>r\<^sub>s\<^sub>o\<^sub>n (oid1) (None) (None) (None))) (\<lfloor>1000\<rfloor>))))))) ((assocs (\<sigma>\<^sub>1))))"
   apply(simp add: \<sigma>\<^sub>1_def oid1_def oid2_def oid4_def oid5_def oid6_def oid9_def)
   apply(subst (1) fun_upd_twist, simp)
   apply(subst (2) fun_upd_twist, simp)
@@ -2931,7 +2940,7 @@ lemma perm_\<sigma>\<^sub>1 : "\<sigma>\<^sub>1 = (state.make ((Map.empty (oid9 
   apply(subst (1) fun_upd_twist, simp)
 by(simp)
 
-(* 133 ************************************ 800 + 12 *)
+(* 136 ************************************ 802 + 12 *)
 lemma \<sigma>\<^sub>1_OclAllInstances_generic_exec_Person : 
 assumes [simp]: "(\<And>a. (pre_post ((mk (a)))) = a)"
 shows "(mk (\<sigma>\<^sub>1)) \<Turnstile> (OclAllInstances_generic (pre_post) (Person)) \<doteq> Set{(\<lambda>_. \<lfloor>\<lfloor>(mkoid\<^sub>P\<^sub>e\<^sub>r\<^sub>s\<^sub>o\<^sub>n ((mk\<^sub>P\<^sub>e\<^sub>r\<^sub>s\<^sub>o\<^sub>n (oid1) (None) (None) (None))) (\<lfloor>1000\<rfloor>))\<rfloor>\<rfloor>) , (\<lambda>_. \<lfloor>\<lfloor>(mkoid\<^sub>P\<^sub>e\<^sub>r\<^sub>s\<^sub>o\<^sub>n ((mk\<^sub>P\<^sub>e\<^sub>r\<^sub>s\<^sub>o\<^sub>n (oid2) (None) (None) (None))) (\<lfloor>1200\<rfloor>))\<rfloor>\<rfloor>) , (\<lambda>_. \<lfloor>\<lfloor>(mkoid\<^sub>P\<^sub>e\<^sub>r\<^sub>s\<^sub>o\<^sub>n ((mk\<^sub>P\<^sub>e\<^sub>r\<^sub>s\<^sub>o\<^sub>n (oid4) (None) (None) (None))) (\<lfloor>2600\<rfloor>))\<rfloor>\<rfloor>) , X\<^sub>P\<^sub>e\<^sub>r\<^sub>s\<^sub>o\<^sub>n5 , (\<lambda>_. \<lfloor>\<lfloor>(mkoid\<^sub>P\<^sub>e\<^sub>r\<^sub>s\<^sub>o\<^sub>n ((mk\<^sub>P\<^sub>e\<^sub>r\<^sub>s\<^sub>o\<^sub>n (oid6) (None) (None) (None))) (\<lfloor>2300\<rfloor>))\<rfloor>\<rfloor>) , X\<^sub>P\<^sub>e\<^sub>r\<^sub>s\<^sub>o\<^sub>n9}"
@@ -3017,18 +3026,22 @@ shows "(\<sigma>\<^sub>1 , st) \<Turnstile> (OclAllInstances_at_pre (OclAny)) \<
   unfolding OclAllInstances_at_pre_def
 by(rule \<sigma>\<^sub>1_OclAllInstances_generic_exec_OclAny, simp) 
 
-(* 134 ************************************ 812 + 1 *)
-definition "\<sigma>\<^sub>1' = (state.make ((Map.empty (oid1 \<mapsto> (in\<^sub>P\<^sub>e\<^sub>r\<^sub>s\<^sub>o\<^sub>n (X\<^sub>P\<^sub>e\<^sub>r\<^sub>s\<^sub>o\<^sub>n1\<^sub>P\<^sub>e\<^sub>r\<^sub>s\<^sub>o\<^sub>n))) (oid2 \<mapsto> (in\<^sub>P\<^sub>e\<^sub>r\<^sub>s\<^sub>o\<^sub>n (X\<^sub>P\<^sub>e\<^sub>r\<^sub>s\<^sub>o\<^sub>n2\<^sub>P\<^sub>e\<^sub>r\<^sub>s\<^sub>o\<^sub>n))) (oid3 \<mapsto> (in\<^sub>P\<^sub>e\<^sub>r\<^sub>s\<^sub>o\<^sub>n (X\<^sub>P\<^sub>e\<^sub>r\<^sub>s\<^sub>o\<^sub>n3\<^sub>P\<^sub>e\<^sub>r\<^sub>s\<^sub>o\<^sub>n))) (oid4 \<mapsto> (in\<^sub>P\<^sub>e\<^sub>r\<^sub>s\<^sub>o\<^sub>n (X\<^sub>P\<^sub>e\<^sub>r\<^sub>s\<^sub>o\<^sub>n4\<^sub>P\<^sub>e\<^sub>r\<^sub>s\<^sub>o\<^sub>n))) (oid6 \<mapsto> (in\<^sub>P\<^sub>e\<^sub>r\<^sub>s\<^sub>o\<^sub>n (X\<^sub>P\<^sub>e\<^sub>r\<^sub>s\<^sub>o\<^sub>n6\<^sub>P\<^sub>e\<^sub>r\<^sub>s\<^sub>o\<^sub>n))) (oid7 \<mapsto> (in\<^sub>O\<^sub>c\<^sub>l\<^sub>A\<^sub>n\<^sub>y (X\<^sub>P\<^sub>e\<^sub>r\<^sub>s\<^sub>o\<^sub>n7\<^sub>O\<^sub>c\<^sub>l\<^sub>A\<^sub>n\<^sub>y))) (oid8 \<mapsto> (in\<^sub>O\<^sub>c\<^sub>l\<^sub>A\<^sub>n\<^sub>y (X\<^sub>P\<^sub>e\<^sub>r\<^sub>s\<^sub>o\<^sub>n8\<^sub>O\<^sub>c\<^sub>l\<^sub>A\<^sub>n\<^sub>y))) (oid9 \<mapsto> (in\<^sub>P\<^sub>e\<^sub>r\<^sub>s\<^sub>o\<^sub>n (X\<^sub>P\<^sub>e\<^sub>r\<^sub>s\<^sub>o\<^sub>n9\<^sub>P\<^sub>e\<^sub>r\<^sub>s\<^sub>o\<^sub>n))))) ((Map.empty (oid\<^sub>P\<^sub>e\<^sub>r\<^sub>s\<^sub>o\<^sub>n\<B>\<O>\<S>\<S> \<mapsto> (Cons ((Pair ((Cons (oid1) (Nil))) ((Cons (oid2) (Nil))))) ((Cons ((Pair ((Cons (oid2) (Nil))) ((Cons (oid2) (Nil))))) ((Cons ((Pair ((Cons (oid6) (Nil))) ((Cons (oid7) (Nil))))) ((Cons ((Pair ((Cons (oid7) (Nil))) ((Cons (oid7) (Nil))))) (Nil))))))))))) ((Map.empty )))"
+(* 137 ************************************ 814 + 0 *)
 
-(* 135 ************************************ 813 + 1 *)
+(* 138 ************************************ 814 + 1 *)
+definition "\<sigma>\<^sub>1' = (state.make ((Map.empty (oid1 \<mapsto> (in\<^sub>P\<^sub>e\<^sub>r\<^sub>s\<^sub>o\<^sub>n (X\<^sub>P\<^sub>e\<^sub>r\<^sub>s\<^sub>o\<^sub>n1\<^sub>P\<^sub>e\<^sub>r\<^sub>s\<^sub>o\<^sub>n))) (oid2 \<mapsto> (in\<^sub>P\<^sub>e\<^sub>r\<^sub>s\<^sub>o\<^sub>n (X\<^sub>P\<^sub>e\<^sub>r\<^sub>s\<^sub>o\<^sub>n2\<^sub>P\<^sub>e\<^sub>r\<^sub>s\<^sub>o\<^sub>n))) (oid3 \<mapsto> (in\<^sub>P\<^sub>e\<^sub>r\<^sub>s\<^sub>o\<^sub>n (X\<^sub>P\<^sub>e\<^sub>r\<^sub>s\<^sub>o\<^sub>n3\<^sub>P\<^sub>e\<^sub>r\<^sub>s\<^sub>o\<^sub>n))) (oid4 \<mapsto> (in\<^sub>P\<^sub>e\<^sub>r\<^sub>s\<^sub>o\<^sub>n (X\<^sub>P\<^sub>e\<^sub>r\<^sub>s\<^sub>o\<^sub>n4\<^sub>P\<^sub>e\<^sub>r\<^sub>s\<^sub>o\<^sub>n))) (oid6 \<mapsto> (in\<^sub>P\<^sub>e\<^sub>r\<^sub>s\<^sub>o\<^sub>n (X\<^sub>P\<^sub>e\<^sub>r\<^sub>s\<^sub>o\<^sub>n6\<^sub>P\<^sub>e\<^sub>r\<^sub>s\<^sub>o\<^sub>n))) (oid7 \<mapsto> (in\<^sub>O\<^sub>c\<^sub>l\<^sub>A\<^sub>n\<^sub>y (X\<^sub>P\<^sub>e\<^sub>r\<^sub>s\<^sub>o\<^sub>n7\<^sub>O\<^sub>c\<^sub>l\<^sub>A\<^sub>n\<^sub>y))) (oid8 \<mapsto> (in\<^sub>O\<^sub>c\<^sub>l\<^sub>A\<^sub>n\<^sub>y (X\<^sub>P\<^sub>e\<^sub>r\<^sub>s\<^sub>o\<^sub>n8\<^sub>O\<^sub>c\<^sub>l\<^sub>A\<^sub>n\<^sub>y))) (oid9 \<mapsto> (in\<^sub>P\<^sub>e\<^sub>r\<^sub>s\<^sub>o\<^sub>n (X\<^sub>P\<^sub>e\<^sub>r\<^sub>s\<^sub>o\<^sub>n9\<^sub>P\<^sub>e\<^sub>r\<^sub>s\<^sub>o\<^sub>n))))) ((map_of_list ([(oid\<^sub>P\<^sub>e\<^sub>r\<^sub>s\<^sub>o\<^sub>n_0_\<B>\<O>\<S>\<S> , (List.map ((\<lambda>(x , y). [x , y]) o switch\<^sub>2_01) ([[[oid1] , [oid2]] , [[oid2] , [oid2]] , [[oid6] , [oid7]] , [[oid7] , [oid7]]])))]))))"
+
+(* 139 ************************************ 815 + 0 *)
+
+(* 140 ************************************ 815 + 1 *)
 lemma dom_\<sigma>\<^sub>1' : "(dom ((heap (\<sigma>\<^sub>1')))) = {oid1 , oid2 , oid3 , oid4 , oid6 , oid7 , oid8 , oid9}"
 by(auto simp: \<sigma>\<^sub>1'_def)
 
-(* 136 ************************************ 814 + 1 *)
+(* 141 ************************************ 816 + 1 *)
 lemmas [simp,code_unfold] = dom_\<sigma>\<^sub>1'
 
-(* 137 ************************************ 815 + 1 *)
-lemma perm_\<sigma>\<^sub>1' : "\<sigma>\<^sub>1' = (state.make ((Map.empty (oid9 \<mapsto> (in\<^sub>P\<^sub>e\<^sub>r\<^sub>s\<^sub>o\<^sub>n (X\<^sub>P\<^sub>e\<^sub>r\<^sub>s\<^sub>o\<^sub>n9\<^sub>P\<^sub>e\<^sub>r\<^sub>s\<^sub>o\<^sub>n))) (oid8 \<mapsto> (in\<^sub>O\<^sub>c\<^sub>l\<^sub>A\<^sub>n\<^sub>y (X\<^sub>P\<^sub>e\<^sub>r\<^sub>s\<^sub>o\<^sub>n8\<^sub>O\<^sub>c\<^sub>l\<^sub>A\<^sub>n\<^sub>y))) (oid7 \<mapsto> (in\<^sub>O\<^sub>c\<^sub>l\<^sub>A\<^sub>n\<^sub>y (X\<^sub>P\<^sub>e\<^sub>r\<^sub>s\<^sub>o\<^sub>n7\<^sub>O\<^sub>c\<^sub>l\<^sub>A\<^sub>n\<^sub>y))) (oid6 \<mapsto> (in\<^sub>P\<^sub>e\<^sub>r\<^sub>s\<^sub>o\<^sub>n (X\<^sub>P\<^sub>e\<^sub>r\<^sub>s\<^sub>o\<^sub>n6\<^sub>P\<^sub>e\<^sub>r\<^sub>s\<^sub>o\<^sub>n))) (oid4 \<mapsto> (in\<^sub>P\<^sub>e\<^sub>r\<^sub>s\<^sub>o\<^sub>n (X\<^sub>P\<^sub>e\<^sub>r\<^sub>s\<^sub>o\<^sub>n4\<^sub>P\<^sub>e\<^sub>r\<^sub>s\<^sub>o\<^sub>n))) (oid3 \<mapsto> (in\<^sub>P\<^sub>e\<^sub>r\<^sub>s\<^sub>o\<^sub>n (X\<^sub>P\<^sub>e\<^sub>r\<^sub>s\<^sub>o\<^sub>n3\<^sub>P\<^sub>e\<^sub>r\<^sub>s\<^sub>o\<^sub>n))) (oid2 \<mapsto> (in\<^sub>P\<^sub>e\<^sub>r\<^sub>s\<^sub>o\<^sub>n (X\<^sub>P\<^sub>e\<^sub>r\<^sub>s\<^sub>o\<^sub>n2\<^sub>P\<^sub>e\<^sub>r\<^sub>s\<^sub>o\<^sub>n))) (oid1 \<mapsto> (in\<^sub>P\<^sub>e\<^sub>r\<^sub>s\<^sub>o\<^sub>n (X\<^sub>P\<^sub>e\<^sub>r\<^sub>s\<^sub>o\<^sub>n1\<^sub>P\<^sub>e\<^sub>r\<^sub>s\<^sub>o\<^sub>n))))) ((assocs\<^sub>2 (\<sigma>\<^sub>1'))) ((assocs\<^sub>3 (\<sigma>\<^sub>1'))))"
+(* 142 ************************************ 817 + 1 *)
+lemma perm_\<sigma>\<^sub>1' : "\<sigma>\<^sub>1' = (state.make ((Map.empty (oid9 \<mapsto> (in\<^sub>P\<^sub>e\<^sub>r\<^sub>s\<^sub>o\<^sub>n (X\<^sub>P\<^sub>e\<^sub>r\<^sub>s\<^sub>o\<^sub>n9\<^sub>P\<^sub>e\<^sub>r\<^sub>s\<^sub>o\<^sub>n))) (oid8 \<mapsto> (in\<^sub>O\<^sub>c\<^sub>l\<^sub>A\<^sub>n\<^sub>y (X\<^sub>P\<^sub>e\<^sub>r\<^sub>s\<^sub>o\<^sub>n8\<^sub>O\<^sub>c\<^sub>l\<^sub>A\<^sub>n\<^sub>y))) (oid7 \<mapsto> (in\<^sub>O\<^sub>c\<^sub>l\<^sub>A\<^sub>n\<^sub>y (X\<^sub>P\<^sub>e\<^sub>r\<^sub>s\<^sub>o\<^sub>n7\<^sub>O\<^sub>c\<^sub>l\<^sub>A\<^sub>n\<^sub>y))) (oid6 \<mapsto> (in\<^sub>P\<^sub>e\<^sub>r\<^sub>s\<^sub>o\<^sub>n (X\<^sub>P\<^sub>e\<^sub>r\<^sub>s\<^sub>o\<^sub>n6\<^sub>P\<^sub>e\<^sub>r\<^sub>s\<^sub>o\<^sub>n))) (oid4 \<mapsto> (in\<^sub>P\<^sub>e\<^sub>r\<^sub>s\<^sub>o\<^sub>n (X\<^sub>P\<^sub>e\<^sub>r\<^sub>s\<^sub>o\<^sub>n4\<^sub>P\<^sub>e\<^sub>r\<^sub>s\<^sub>o\<^sub>n))) (oid3 \<mapsto> (in\<^sub>P\<^sub>e\<^sub>r\<^sub>s\<^sub>o\<^sub>n (X\<^sub>P\<^sub>e\<^sub>r\<^sub>s\<^sub>o\<^sub>n3\<^sub>P\<^sub>e\<^sub>r\<^sub>s\<^sub>o\<^sub>n))) (oid2 \<mapsto> (in\<^sub>P\<^sub>e\<^sub>r\<^sub>s\<^sub>o\<^sub>n (X\<^sub>P\<^sub>e\<^sub>r\<^sub>s\<^sub>o\<^sub>n2\<^sub>P\<^sub>e\<^sub>r\<^sub>s\<^sub>o\<^sub>n))) (oid1 \<mapsto> (in\<^sub>P\<^sub>e\<^sub>r\<^sub>s\<^sub>o\<^sub>n (X\<^sub>P\<^sub>e\<^sub>r\<^sub>s\<^sub>o\<^sub>n1\<^sub>P\<^sub>e\<^sub>r\<^sub>s\<^sub>o\<^sub>n))))) ((assocs (\<sigma>\<^sub>1'))))"
   apply(simp add: \<sigma>\<^sub>1'_def oid1_def oid2_def oid3_def oid4_def oid6_def oid7_def oid8_def oid9_def)
   apply(subst (1) fun_upd_twist, simp)
   apply(subst (2) fun_upd_twist, simp)
@@ -3060,7 +3073,7 @@ lemma perm_\<sigma>\<^sub>1' : "\<sigma>\<^sub>1' = (state.make ((Map.empty (oid
   apply(subst (1) fun_upd_twist, simp)
 by(simp)
 
-(* 138 ************************************ 816 + 12 *)
+(* 143 ************************************ 818 + 12 *)
 lemma \<sigma>\<^sub>1'_OclAllInstances_generic_exec_Person : 
 assumes [simp]: "(\<And>a. (pre_post ((mk (a)))) = a)"
 shows "(mk (\<sigma>\<^sub>1')) \<Turnstile> (OclAllInstances_generic (pre_post) (Person)) \<doteq> Set{X\<^sub>P\<^sub>e\<^sub>r\<^sub>s\<^sub>o\<^sub>n1 , X\<^sub>P\<^sub>e\<^sub>r\<^sub>s\<^sub>o\<^sub>n2 , X\<^sub>P\<^sub>e\<^sub>r\<^sub>s\<^sub>o\<^sub>n3 , X\<^sub>P\<^sub>e\<^sub>r\<^sub>s\<^sub>o\<^sub>n4 , X\<^sub>P\<^sub>e\<^sub>r\<^sub>s\<^sub>o\<^sub>n6 , X\<^sub>P\<^sub>e\<^sub>r\<^sub>s\<^sub>o\<^sub>n7 .oclAsType(Person) , X\<^sub>P\<^sub>e\<^sub>r\<^sub>s\<^sub>o\<^sub>n9}"
@@ -3154,21 +3167,25 @@ shows "(\<sigma>\<^sub>1' , st) \<Turnstile> (OclAllInstances_at_pre (OclAny)) \
   unfolding OclAllInstances_at_pre_def
 by(rule \<sigma>\<^sub>1'_OclAllInstances_generic_exec_OclAny, simp) 
 
-(* 139 ************************************ 828 + 1 *)
-definition "\<sigma>\<^sub>0 = (state.make ((Map.empty )) ((Map.empty )) ((Map.empty )))"
+(* 144 ************************************ 830 + 0 *)
 
-(* 140 ************************************ 829 + 1 *)
+(* 145 ************************************ 830 + 1 *)
+definition "\<sigma>\<^sub>0 = (state.make ((Map.empty )) ((map_of_list ([]))))"
+
+(* 146 ************************************ 831 + 0 *)
+
+(* 147 ************************************ 831 + 1 *)
 lemma dom_\<sigma>\<^sub>0 : "(dom ((heap (\<sigma>\<^sub>0)))) = {}"
 by(auto simp: \<sigma>\<^sub>0_def)
 
-(* 141 ************************************ 830 + 1 *)
+(* 148 ************************************ 832 + 1 *)
 lemmas [simp,code_unfold] = dom_\<sigma>\<^sub>0
 
-(* 142 ************************************ 831 + 1 *)
-lemma perm_\<sigma>\<^sub>0 : "\<sigma>\<^sub>0 = (state.make ((Map.empty )) ((assocs\<^sub>2 (\<sigma>\<^sub>0))) ((assocs\<^sub>3 (\<sigma>\<^sub>0))))"
+(* 149 ************************************ 833 + 1 *)
+lemma perm_\<sigma>\<^sub>0 : "\<sigma>\<^sub>0 = (state.make ((Map.empty )) ((assocs (\<sigma>\<^sub>0))))"
 by(simp add: \<sigma>\<^sub>0_def)
 
-(* 143 ************************************ 832 + 12 *)
+(* 150 ************************************ 834 + 12 *)
 lemma \<sigma>\<^sub>0_OclAllInstances_generic_exec_Person : 
 assumes [simp]: "(\<And>a. (pre_post ((mk (a)))) = a)"
 shows "(mk (\<sigma>\<^sub>0)) \<Turnstile> (OclAllInstances_generic (pre_post) (Person)) \<doteq> Set{}"
@@ -3230,28 +3247,30 @@ shows "(\<sigma>\<^sub>0 , st) \<Turnstile> (OclAllInstances_at_pre (OclAny)) \<
   unfolding OclAllInstances_at_pre_def
 by(rule \<sigma>\<^sub>0_OclAllInstances_generic_exec_OclAny, simp) 
 
-(* 144 ************************************ 844 + 1 *)
+(* 151 ************************************ 846 + 1 *)
 lemma basic_\<sigma>\<^sub>1_\<sigma>\<^sub>1'_wff : "(WFF ((\<sigma>\<^sub>1 , \<sigma>\<^sub>1')))"
 by(simp add: WFF_def \<sigma>\<^sub>1_def \<sigma>\<^sub>1'_def oid_of_\<AA>_def oid1_def oid2_def oid3_def oid4_def oid5_def oid6_def oid7_def oid8_def oid9_def X\<^sub>P\<^sub>e\<^sub>r\<^sub>s\<^sub>o\<^sub>n1\<^sub>P\<^sub>e\<^sub>r\<^sub>s\<^sub>o\<^sub>n_def X\<^sub>P\<^sub>e\<^sub>r\<^sub>s\<^sub>o\<^sub>n2\<^sub>P\<^sub>e\<^sub>r\<^sub>s\<^sub>o\<^sub>n_def X\<^sub>P\<^sub>e\<^sub>r\<^sub>s\<^sub>o\<^sub>n3\<^sub>P\<^sub>e\<^sub>r\<^sub>s\<^sub>o\<^sub>n_def X\<^sub>P\<^sub>e\<^sub>r\<^sub>s\<^sub>o\<^sub>n4\<^sub>P\<^sub>e\<^sub>r\<^sub>s\<^sub>o\<^sub>n_def X\<^sub>P\<^sub>e\<^sub>r\<^sub>s\<^sub>o\<^sub>n5\<^sub>P\<^sub>e\<^sub>r\<^sub>s\<^sub>o\<^sub>n_def X\<^sub>P\<^sub>e\<^sub>r\<^sub>s\<^sub>o\<^sub>n6\<^sub>P\<^sub>e\<^sub>r\<^sub>s\<^sub>o\<^sub>n_def X\<^sub>P\<^sub>e\<^sub>r\<^sub>s\<^sub>o\<^sub>n7\<^sub>O\<^sub>c\<^sub>l\<^sub>A\<^sub>n\<^sub>y_def X\<^sub>P\<^sub>e\<^sub>r\<^sub>s\<^sub>o\<^sub>n8\<^sub>O\<^sub>c\<^sub>l\<^sub>A\<^sub>n\<^sub>y_def X\<^sub>P\<^sub>e\<^sub>r\<^sub>s\<^sub>o\<^sub>n9\<^sub>P\<^sub>e\<^sub>r\<^sub>s\<^sub>o\<^sub>n_def oid_of_typeoid\<^sub>O\<^sub>c\<^sub>l\<^sub>A\<^sub>n\<^sub>y_def oid_of_typeoid\<^sub>P\<^sub>e\<^sub>r\<^sub>s\<^sub>o\<^sub>n_def)
 
-(* 145 ************************************ 845 + 9 *)
-lemma oid1_OclIsMaintained : "(\<sigma>\<^sub>1 , \<sigma>\<^sub>1') \<Turnstile> (OclIsMaintained (X\<^sub>P\<^sub>e\<^sub>r\<^sub>s\<^sub>o\<^sub>n1))"
+(* 152 ************************************ 847 + 10 *)
+lemma oid1\<sigma>\<^sub>1\<sigma>\<^sub>1'_\<sigma>\<^sub>1'_OclIsMaintained : "(\<sigma>\<^sub>1 , \<sigma>\<^sub>1') \<Turnstile> (OclIsMaintained (X\<^sub>P\<^sub>e\<^sub>r\<^sub>s\<^sub>o\<^sub>n1))"
 by(simp add: X\<^sub>P\<^sub>e\<^sub>r\<^sub>s\<^sub>o\<^sub>n1_def X\<^sub>P\<^sub>e\<^sub>r\<^sub>s\<^sub>o\<^sub>n1\<^sub>P\<^sub>e\<^sub>r\<^sub>s\<^sub>o\<^sub>n_def OclIsMaintained_def OclValid_def \<sigma>\<^sub>1_def \<sigma>\<^sub>1'_def oid_of_option_def oid1_def oid2_def oid3_def oid4_def oid5_def oid6_def oid7_def oid8_def oid9_def oid_of_typeoid\<^sub>O\<^sub>c\<^sub>l\<^sub>A\<^sub>n\<^sub>y_def oid_of_typeoid\<^sub>P\<^sub>e\<^sub>r\<^sub>s\<^sub>o\<^sub>n_def)
-lemma oid2_OclIsMaintained : "(\<sigma>\<^sub>1 , \<sigma>\<^sub>1') \<Turnstile> (OclIsMaintained (X\<^sub>P\<^sub>e\<^sub>r\<^sub>s\<^sub>o\<^sub>n2))"
+lemma oid2\<sigma>\<^sub>1\<sigma>\<^sub>1'_\<sigma>\<^sub>1'_OclIsMaintained : "(\<sigma>\<^sub>1 , \<sigma>\<^sub>1') \<Turnstile> (OclIsMaintained (X\<^sub>P\<^sub>e\<^sub>r\<^sub>s\<^sub>o\<^sub>n2))"
 by(simp add: X\<^sub>P\<^sub>e\<^sub>r\<^sub>s\<^sub>o\<^sub>n2_def X\<^sub>P\<^sub>e\<^sub>r\<^sub>s\<^sub>o\<^sub>n2\<^sub>P\<^sub>e\<^sub>r\<^sub>s\<^sub>o\<^sub>n_def OclIsMaintained_def OclValid_def \<sigma>\<^sub>1_def \<sigma>\<^sub>1'_def oid_of_option_def oid1_def oid2_def oid3_def oid4_def oid5_def oid6_def oid7_def oid8_def oid9_def oid_of_typeoid\<^sub>O\<^sub>c\<^sub>l\<^sub>A\<^sub>n\<^sub>y_def oid_of_typeoid\<^sub>P\<^sub>e\<^sub>r\<^sub>s\<^sub>o\<^sub>n_def)
-lemma oid3_OclIsNew : "(\<sigma>\<^sub>1 , \<sigma>\<^sub>1') \<Turnstile> (OclIsNew (X\<^sub>P\<^sub>e\<^sub>r\<^sub>s\<^sub>o\<^sub>n3))"
+lemma oid3\<sigma>\<^sub>1\<sigma>\<^sub>1'_\<sigma>\<^sub>1'_OclIsNew : "(\<sigma>\<^sub>1 , \<sigma>\<^sub>1') \<Turnstile> (OclIsNew (X\<^sub>P\<^sub>e\<^sub>r\<^sub>s\<^sub>o\<^sub>n3))"
 by(simp add: X\<^sub>P\<^sub>e\<^sub>r\<^sub>s\<^sub>o\<^sub>n3_def X\<^sub>P\<^sub>e\<^sub>r\<^sub>s\<^sub>o\<^sub>n3\<^sub>P\<^sub>e\<^sub>r\<^sub>s\<^sub>o\<^sub>n_def OclIsNew_def OclValid_def \<sigma>\<^sub>1_def \<sigma>\<^sub>1'_def oid_of_option_def oid1_def oid2_def oid3_def oid4_def oid5_def oid6_def oid7_def oid8_def oid9_def oid_of_typeoid\<^sub>O\<^sub>c\<^sub>l\<^sub>A\<^sub>n\<^sub>y_def oid_of_typeoid\<^sub>P\<^sub>e\<^sub>r\<^sub>s\<^sub>o\<^sub>n_def)
-lemma oid4_OclIsMaintained : "(\<sigma>\<^sub>1 , \<sigma>\<^sub>1') \<Turnstile> (OclIsMaintained (X\<^sub>P\<^sub>e\<^sub>r\<^sub>s\<^sub>o\<^sub>n4))"
+lemma oid4\<sigma>\<^sub>1\<sigma>\<^sub>1'_\<sigma>\<^sub>1'_OclIsMaintained : "(\<sigma>\<^sub>1 , \<sigma>\<^sub>1') \<Turnstile> (OclIsMaintained (X\<^sub>P\<^sub>e\<^sub>r\<^sub>s\<^sub>o\<^sub>n4))"
 by(simp add: X\<^sub>P\<^sub>e\<^sub>r\<^sub>s\<^sub>o\<^sub>n4_def X\<^sub>P\<^sub>e\<^sub>r\<^sub>s\<^sub>o\<^sub>n4\<^sub>P\<^sub>e\<^sub>r\<^sub>s\<^sub>o\<^sub>n_def OclIsMaintained_def OclValid_def \<sigma>\<^sub>1_def \<sigma>\<^sub>1'_def oid_of_option_def oid1_def oid2_def oid3_def oid4_def oid5_def oid6_def oid7_def oid8_def oid9_def oid_of_typeoid\<^sub>O\<^sub>c\<^sub>l\<^sub>A\<^sub>n\<^sub>y_def oid_of_typeoid\<^sub>P\<^sub>e\<^sub>r\<^sub>s\<^sub>o\<^sub>n_def)
-lemma oid5_OclIsDeleted : "(\<sigma>\<^sub>1 , \<sigma>\<^sub>1') \<Turnstile> (OclIsDeleted (X\<^sub>P\<^sub>e\<^sub>r\<^sub>s\<^sub>o\<^sub>n5))"
+lemma oid5\<sigma>\<^sub>1\<sigma>\<^sub>1'_\<sigma>\<^sub>1_OclIsDeleted : "(\<sigma>\<^sub>1 , \<sigma>\<^sub>1') \<Turnstile> (OclIsDeleted (X\<^sub>P\<^sub>e\<^sub>r\<^sub>s\<^sub>o\<^sub>n5))"
 by(simp add: X\<^sub>P\<^sub>e\<^sub>r\<^sub>s\<^sub>o\<^sub>n5_def X\<^sub>P\<^sub>e\<^sub>r\<^sub>s\<^sub>o\<^sub>n5\<^sub>P\<^sub>e\<^sub>r\<^sub>s\<^sub>o\<^sub>n_def OclIsDeleted_def OclValid_def \<sigma>\<^sub>1_def \<sigma>\<^sub>1'_def oid_of_option_def oid1_def oid2_def oid3_def oid4_def oid5_def oid6_def oid7_def oid8_def oid9_def oid_of_typeoid\<^sub>O\<^sub>c\<^sub>l\<^sub>A\<^sub>n\<^sub>y_def oid_of_typeoid\<^sub>P\<^sub>e\<^sub>r\<^sub>s\<^sub>o\<^sub>n_def)
-lemma oid6_OclIsMaintained : "(\<sigma>\<^sub>1 , \<sigma>\<^sub>1') \<Turnstile> (OclIsMaintained (X\<^sub>P\<^sub>e\<^sub>r\<^sub>s\<^sub>o\<^sub>n6))"
+lemma oid6\<sigma>\<^sub>1\<sigma>\<^sub>1'_\<sigma>\<^sub>1'_OclIsMaintained : "(\<sigma>\<^sub>1 , \<sigma>\<^sub>1') \<Turnstile> (OclIsMaintained (X\<^sub>P\<^sub>e\<^sub>r\<^sub>s\<^sub>o\<^sub>n6))"
 by(simp add: X\<^sub>P\<^sub>e\<^sub>r\<^sub>s\<^sub>o\<^sub>n6_def X\<^sub>P\<^sub>e\<^sub>r\<^sub>s\<^sub>o\<^sub>n6\<^sub>P\<^sub>e\<^sub>r\<^sub>s\<^sub>o\<^sub>n_def OclIsMaintained_def OclValid_def \<sigma>\<^sub>1_def \<sigma>\<^sub>1'_def oid_of_option_def oid1_def oid2_def oid3_def oid4_def oid5_def oid6_def oid7_def oid8_def oid9_def oid_of_typeoid\<^sub>O\<^sub>c\<^sub>l\<^sub>A\<^sub>n\<^sub>y_def oid_of_typeoid\<^sub>P\<^sub>e\<^sub>r\<^sub>s\<^sub>o\<^sub>n_def)
-lemma oid7_OclIsNew : "(\<sigma>\<^sub>1 , \<sigma>\<^sub>1') \<Turnstile> (OclIsNew (X\<^sub>P\<^sub>e\<^sub>r\<^sub>s\<^sub>o\<^sub>n7))"
+lemma oid7\<sigma>\<^sub>1\<sigma>\<^sub>1'_\<sigma>\<^sub>1'_OclIsNew : "(\<sigma>\<^sub>1 , \<sigma>\<^sub>1') \<Turnstile> (OclIsNew (X\<^sub>P\<^sub>e\<^sub>r\<^sub>s\<^sub>o\<^sub>n7))"
 by(simp add: X\<^sub>P\<^sub>e\<^sub>r\<^sub>s\<^sub>o\<^sub>n7_def X\<^sub>P\<^sub>e\<^sub>r\<^sub>s\<^sub>o\<^sub>n7\<^sub>O\<^sub>c\<^sub>l\<^sub>A\<^sub>n\<^sub>y_def OclIsNew_def OclValid_def \<sigma>\<^sub>1_def \<sigma>\<^sub>1'_def oid_of_option_def oid1_def oid2_def oid3_def oid4_def oid5_def oid6_def oid7_def oid8_def oid9_def oid_of_typeoid\<^sub>O\<^sub>c\<^sub>l\<^sub>A\<^sub>n\<^sub>y_def oid_of_typeoid\<^sub>P\<^sub>e\<^sub>r\<^sub>s\<^sub>o\<^sub>n_def)
-lemma oid8_OclIsNew : "(\<sigma>\<^sub>1 , \<sigma>\<^sub>1') \<Turnstile> (OclIsNew (X\<^sub>P\<^sub>e\<^sub>r\<^sub>s\<^sub>o\<^sub>n8))"
+lemma oid8\<sigma>\<^sub>1\<sigma>\<^sub>1'_\<sigma>\<^sub>1'_OclIsNew : "(\<sigma>\<^sub>1 , \<sigma>\<^sub>1') \<Turnstile> (OclIsNew (X\<^sub>P\<^sub>e\<^sub>r\<^sub>s\<^sub>o\<^sub>n8))"
 by(simp add: X\<^sub>P\<^sub>e\<^sub>r\<^sub>s\<^sub>o\<^sub>n8_def X\<^sub>P\<^sub>e\<^sub>r\<^sub>s\<^sub>o\<^sub>n8\<^sub>O\<^sub>c\<^sub>l\<^sub>A\<^sub>n\<^sub>y_def OclIsNew_def OclValid_def \<sigma>\<^sub>1_def \<sigma>\<^sub>1'_def oid_of_option_def oid1_def oid2_def oid3_def oid4_def oid5_def oid6_def oid7_def oid8_def oid9_def oid_of_typeoid\<^sub>O\<^sub>c\<^sub>l\<^sub>A\<^sub>n\<^sub>y_def oid_of_typeoid\<^sub>P\<^sub>e\<^sub>r\<^sub>s\<^sub>o\<^sub>n_def)
-lemma oid9_OclIsMaintained : "(\<sigma>\<^sub>1 , \<sigma>\<^sub>1') \<Turnstile> (OclIsMaintained (X\<^sub>P\<^sub>e\<^sub>r\<^sub>s\<^sub>o\<^sub>n9))"
+lemma oid9\<sigma>\<^sub>1\<sigma>\<^sub>1'_\<sigma>\<^sub>1_OclIsMaintained : "(\<sigma>\<^sub>1 , \<sigma>\<^sub>1') \<Turnstile> (OclIsMaintained (X\<^sub>P\<^sub>e\<^sub>r\<^sub>s\<^sub>o\<^sub>n9))"
+by(simp add: X\<^sub>P\<^sub>e\<^sub>r\<^sub>s\<^sub>o\<^sub>n9_def X\<^sub>P\<^sub>e\<^sub>r\<^sub>s\<^sub>o\<^sub>n9\<^sub>P\<^sub>e\<^sub>r\<^sub>s\<^sub>o\<^sub>n_def OclIsMaintained_def OclValid_def \<sigma>\<^sub>1_def \<sigma>\<^sub>1'_def oid_of_option_def oid1_def oid2_def oid3_def oid4_def oid5_def oid6_def oid7_def oid8_def oid9_def oid_of_typeoid\<^sub>O\<^sub>c\<^sub>l\<^sub>A\<^sub>n\<^sub>y_def oid_of_typeoid\<^sub>P\<^sub>e\<^sub>r\<^sub>s\<^sub>o\<^sub>n_def)
+lemma oid9\<sigma>\<^sub>1\<sigma>\<^sub>1'_\<sigma>\<^sub>1'_OclIsMaintained : "(\<sigma>\<^sub>1 , \<sigma>\<^sub>1') \<Turnstile> (OclIsMaintained (X\<^sub>P\<^sub>e\<^sub>r\<^sub>s\<^sub>o\<^sub>n9))"
 by(simp add: X\<^sub>P\<^sub>e\<^sub>r\<^sub>s\<^sub>o\<^sub>n9_def X\<^sub>P\<^sub>e\<^sub>r\<^sub>s\<^sub>o\<^sub>n9\<^sub>P\<^sub>e\<^sub>r\<^sub>s\<^sub>o\<^sub>n_def OclIsMaintained_def OclValid_def \<sigma>\<^sub>1_def \<sigma>\<^sub>1'_def oid_of_option_def oid1_def oid2_def oid3_def oid4_def oid5_def oid6_def oid7_def oid8_def oid9_def oid_of_typeoid\<^sub>O\<^sub>c\<^sub>l\<^sub>A\<^sub>n\<^sub>y_def oid_of_typeoid\<^sub>P\<^sub>e\<^sub>r\<^sub>s\<^sub>o\<^sub>n_def)
 
 end
